src/Lean/Parser/Extension.lean
@@ -372,7 +372,7 @@ def leadingIdentBehavior (env : Environment) (catName : Name) : LeadingIdentBeha
 
 unsafe def evalParserConstUnsafe (declName : Name) (evalFallback? : Option ParserFn := none) : ParserFn := fun ctx s => unsafeBaseIO do
   let categories := (parserExtension.getState ctx.env).categories
-  match (← (mkParserOfConstant categories declName { env := ctx.env, opts := ctx.options }).toBaseIO) with
+  match (← ((mkParserOfConstant categories declName).run { env := ctx.env, opts := ctx.options }).toBaseIO) with
   | .ok (_, p) =>
     -- We should manually register `p`'s tokens before invoking it as it might not be part of any syntax category (yet)
     return adaptUncacheableContextFn (fun ctx => { ctx with tokens := p.info.collectTokens [] |>.foldl (fun tks tk => tks.insert tk tk) ctx.tokens }) p.fn ctx s
