src/Std/Sync/Mutex.lean
@@ -139,7 +139,7 @@ def Mutex.atomically [Monad m] [MonadLiftT BaseIO m] [MonadFinally m]
     (mutex : Mutex α) (k : AtomicT α m β) : m β := do
   try
     mutex.mutex.lock
-    k mutex.ref
+    ReaderT.run k mutex.ref
   finally
     mutex.mutex.unlock
 
@@ -155,7 +155,7 @@ def Mutex.tryAtomically [Monad m] [MonadLiftT BaseIO m] [MonadFinally m]
     (mutex : Mutex α) (k : AtomicT α m β) : m (Option β) := do
   if ← mutex.mutex.tryLock then
     try
-      some <$> k mutex.ref
+      some <$> ReaderT.run k mutex.ref
     finally
       mutex.mutex.unlock
   else
