tests/elab/casesOnSameCtor.lean
@@ -146,15 +146,15 @@ trace: [Compiler.saveMono] size: 5
       | EST.Out.error a.15 a.16 =>
         return _x.11
 [Compiler.saveMono] size: 7
-    def _private.elab.casesOnSameCtor.0._eval @&a @&a _y.1 : EST.Out Exception lcAny PUnit :=
-      let _x.2 := "List";
-      let _x.3 := "match_on_same_ctor";
-      let _x.4 := Name.mkStr2 _x.2 _x.3;
-      let _x.5 := Name.mkStr1 _x.2;
-      let _x.6 := PUnit.unit;
-      let _f.7 := _eval._lam_0 _x.4 _x.5 _x.6;
-      let _x.8 := Lean.Elab.Command.liftTermElabM._redArg _f.7 a a _y.1;
-      return _x.8
+    def _private.elab.casesOnSameCtor.0._eval @&_y.1 @&_y.2 _y.3 : EST.Out Exception lcAny PUnit :=
+      let _x.4 := "List";
+      let _x.5 := "match_on_same_ctor";
+      let _x.6 := Name.mkStr2 _x.4 _x.5;
+      let _x.7 := Name.mkStr1 _x.4;
+      let _x.8 := PUnit.unit;
+      let _f.9 := _eval._lam_0 _x.6 _x.7 _x.8;
+      let _x.10 := Lean.Elab.Command.liftTermElabM._redArg _f.9 _y.1 _y.2 _y.3;
+      return _x.10
 -/
 #guard_msgs in
 set_option trace.Compiler.saveMono true in
